A12Kernel/Proofs.lean
@@ -196,6 +196,7 @@ import A12Kernel.Proofs.ValueList
 import A12Kernel.Proofs.FirstFilledValue
 import A12Kernel.Proofs.BooleanFirstFilledComputation
 import A12Kernel.Proofs.AddressedBooleanFirstFilledComputation
+import A12Kernel.Proofs.AddressedNumberFirstFilledComputation
 import A12Kernel.Proofs.ExactTokenComputationResult
 import A12Kernel.Proofs.CustomFirstFilledComputation
 import A12Kernel.Proofs.AddressedCustomFirstFilledComputation
